for loop

Array.thy
@@ -8,19 +8,19 @@ definition interval :: "nat \<Rightarrow> nat \<Rightarrow> nat set" where
   "interval k l \<equiv> {i. k \<le> i \<and> i \<le> l}"
 
 (* Sum from offset the number of value n *)
-primrec array_sum :: "nat \<Rightarrow> nat \<Rightarrow> 'a array \<Rightarrow> 'a :: {plus, zero}" where
-  "array_sum off 0 a = 0"
-| "array_sum off (Suc n) a = a (off + n) + array_sum off n a"
+primrec array_sum :: "'a array \<Rightarrow> nat \<Rightarrow> nat \<Rightarrow>  'a :: {plus, zero}" where
+  "array_sum a off 0 = 0"
+| "array_sum a off (Suc n) = a (off + n) + array_sum a off n"
 
-fun array_sorted :: "nat \<Rightarrow> nat \<Rightarrow> 'a :: order array \<Rightarrow> bool" where
-  "array_sorted off 0 a \<longleftrightarrow> True"
-| "array_sorted off (Suc 0) a \<longleftrightarrow> True" 
-| "array_sorted off (Suc (Suc n)) a \<longleftrightarrow> a (off + n) \<le> a (off + Suc n) \<and> array_sorted off (Suc n) a"
+fun array_sorted :: "'a :: order array \<Rightarrow> nat \<Rightarrow> nat \<Rightarrow> bool" where
+  "array_sorted a off 0 \<longleftrightarrow> True"
+| "array_sorted a off (Suc 0) \<longleftrightarrow> True" 
+| "array_sorted a off (Suc (Suc n)) \<longleftrightarrow> a (off + n) \<le> a (off + Suc n) \<and> array_sorted a off (Suc n)"
 
 fun new_array :: "'a list \<Rightarrow> 'a array" where
   "new_array xs = nth xs"
 
-lemma "array_sorted i n a \<Longrightarrow> array_sorted (Suc i) (n - 1) a"
+lemma "array_sorted a i n \<Longrightarrow> array_sorted a (Suc i) (n - 1)"
   apply (induct n)
   apply auto
   apply (case_tac n)
@@ -28,19 +28,41 @@ lemma "array_sorted i n a \<Longrightarrow> array_sorted (Suc i) (n - 1) a"
   apply (case_tac nat)
 by auto
 
-lemma last_num: "array_sorted i (Suc (Suc n)) a \<Longrightarrow> a (i + n) \<le> a (i + Suc n)"
+lemma last_num: "n > 0 \<Longrightarrow> array_sorted a i (Suc n) \<Longrightarrow> a (i + n - Suc 0) \<le> a (i + n)"
   by (cases n) auto
 
-lemma "i > 0  \<Longrightarrow> array_sorted i (Suc (Suc n)) a \<Longrightarrow> array_sorted (i - 1) (Suc (Suc (Suc n))) a"
+lemma tt: "i > 0 \<Longrightarrow> \<forall>k \<le> i. a(k) \<le> a(i) \<Longrightarrow> array_sorted a i (n - 1) \<Longrightarrow> array_sorted a (i - 1) n"
 apply (induct n)
-apply simp
-apply force
 apply auto
-apply (cases n)
+apply (case_tac n)
 apply force
-apply (subgoal_tac 
+apply simp
+apply (rule conjI)
+apply (case_tac nat)
+apply simp
+apply (rule last_num)
+apply simp
+apply simp
+apply (case_tac nat)
+apply auto
+done
 
-value "array_sorted 1 2 (new_array [2, 2, 1 :: nat])"
+lemma tt2: "i > 0 \<Longrightarrow> \<forall>k. 1 \<le> k \<and> k \<le> i \<longrightarrow> a(k) \<le> a(i + 1) \<Longrightarrow> array_sorted a (Suc i) n \<Longrightarrow> array_sorted a i (Suc n)"
+apply (induct n)
+apply auto
+apply (case_tac n)
+apply force
+apply simp
+apply (case_tac n)
+apply force
+apply simp
+done
+
+lemma "i > 0 \<Longrightarrow> \<forall>k \<le> i. a(k) \<le> a(i) \<Longrightarrow> array_sorted a i (Suc (Suc n)) \<Longrightarrow> array_sorted a  (i - 1) (Suc (Suc (Suc n)))"
+apply (induct n)
+by auto
+
+value "array_sorted (new_array [2, 2, 1 :: nat]) 1 2"
 
 
 end
